raft/simulator/raft/RaftTest.v
@@ -15,6 +15,132 @@ Import RecordSetNotations.
 
 Section RaftTestInstance.
 
+  (*! Define the test instance !*)
+  (** Time **)
+  Definition time_I_type : Set := unit.
+  Definition time_I_get_time : unit -> time_I_type := fun _ => tt.
+  Definition time_I_sub : time_I_type -> time_I_type -> time_I_type := fun _ _ => tt.
+  Definition time_I_2string : time_I_type -> string := fun _ => "".
+
+  Global Instance TIME_I : Time.
+  Proof.
+    exists time_I_type.
+    { exact time_I_get_time. }
+    { exact time_I_sub. }
+    { exact time_I_2string. }
+  Defined.
+
+  (*! Realization of the context definitions !*)
+  Definition Faults := 1.
+  Definition Clients := 0. (* client is c + 1 *)
+  (* Numbers of replicas *)
+  Definition num_replicas (F : nat) : nat := 3 * F + 1.
+  (* The set of replicas based on the replica numbers *)
+  Definition raft_replicas (F : nat) : Set := nat_n (num_replicas Faults).
+  (* Show decidable equality *)
+  Lemma replica_deq (F : nat) : Deq (raft_replicas F).
+  Proof.
+    apply nat_n_deq.
+  Defined.
+  (* Mapping between the number of a replica and the replica itself *)
+  Definition reps2nat (F : nat) : raft_replicas F -> nat_n (num_replicas Faults) := fun n => n.
+  (* proof reps2nat is bijective *)
+  Lemma bijective_reps2nat (F : nat) : bijective (reps2nat F).
+  Proof.
+    exists (fun n : nat_n (num_replicas Faults) => n); introv; unfold reps2nat; auto.
+    Defined.
+  Definition nclients (C : nat) := S C.
+  Definition raft_client (C : nat) : Set := nat_n (nclients C).
+  Definition client0 (C : nat) : raft_client C.
+  Proof.
+    exists 0. apply leb_correct. unfold nclients. omega.
+  Defined.
+  (* proof client decidability *)
+  Lemma client_deq (C : nat) : Deq (raft_client C).
+  Proof.
+    apply nat_n_deq.
+  Defined.
+  Definition clients2nat (C : nat) : raft_client C -> nat_n (nclients C) := fun n => n.
+  Lemma bijective_clients2nat (C : nat) : bijective (clients2nat C).
+  Proof.
+    exists (fun n : nat_n (nclients C) => n); introv; unfold clients2nat; auto.
+  Defined.
+
+  (*! Raft state machine !*)
+  (** A simple state machine which only adds natural numbers **)
+  Definition rstate : Set := nat.
+  Definition rstate0 : rstate := 0.
+  Definition rresult : Set := nat.
+  Definition rcontent : Set := nat.
+  Definition rupdate (s : rstate) (c : rcontent) : rstate * rresult := (s + c, s + c).
+  Definition nat2string (n : nat) : string := "-". (* used in OCaml *)
+  Global Instance Raft_I_context : RaftContext :=
+    MkRaftContext
+      Faults
+      (raft_replicas Faults)
+      (replica_deq Faults)
+      (reps2nat Faults)
+      (bijective_reps2nat Faults)
+      (nclients Clients)
+      (raft_client Clients)
+      (client_deq Clients)
+      (clients2nat Clients)
+      (bijective_clients2nat Clients)
+      rcontent
+      nat2string
+      rresult
+      rstate
+      rstate0
+      rupdate.
+
+  (*! Tests !*)
+  (** Some tests for the most important parts of the raft protocol to validaty logical
+   ** correctness. Through the number of faults to tolerate we know that there are 4
+   ** nodes in the network. Assign the first as one as leader **)
+  Definition leader : RaftState := to_leader state0 replica0.
+
+  (*! Test the next and match index !*)
+  Print replica0.
+  Compute rep_deq replica0 replica0.
+  Compute (decrease_next_index (next_index0 replica0 1) replica0).
+  Definition leader_inc := (incr_next_index_all leader).
+  Compute gni (node_state leader_inc).
+  Compute decrease_next_index (gni (node_state leader_inc)) replica0.
+
+  (*! Test the log !*)
+  Definition log1 := add2log [] [(new_term_entry term0)].
+  Compute log1.
+  Definition log2 := add2log log1 [(new_content_entry term0 3), (new_content_entry term0 4)].
+  Compute log2.  (* three elements list *)
+  Compute  get_log_entry log2 2.
+  Definition s := new_session [] (client0 0).
+  Definition log3 := add2log log2
+                             [(new_term_entry (term 1)),
+                              (new_sessions_entry (term 1) (fst s)),
+                              (new_content_entry (term 1) 5)].
+  Compute log3. 
+  Compute get_last_entry log3. (* return content entry 5 *)
+  Compute last_session log3. (* get the last session *) 
+  Compute take_from_log log3 2. (* remove last two added entries *)
+  Compute check_entry_term log3 6 (term 1). (* check that content entry 5 is valid *)
+
+  (* test fix_log function 5 entries, term 1 *)
+  Compute log3.
+  Definition l := (update_log leader log3).
+  (* the position 5 is free so just add the new content *)
+  Compute (log (fix_log l [(new_content_entry (term 1) 6)] 5 (term 1))).
+  (* the logs are considered equal since position 4 has term 1 *)
+  Compute (log (fix_log l [(new_content_entry (term 1) 6)] 4 (term 1))).
+  (* the logs are considered unequal since the position 4 has not term 0 *)
+  Compute (log (fix_log l [(new_content_entry (term 1) 6)] 4 (term 0))).
+  (* the logs are considered unequal *)
+  Compute (log (fix_log l [(new_content_entry (term 1) 6)] 3 (term 0))).
+
+  (*! Test the caching !*)
+  Definition cache := add2cache [] session_id0 request_id0 1.
+  Compute cache.
+  Compute add_result2cache cache 1 3.
+  Compute get_cached_result (add_result2cache cache 1 3) session_id0 request_id0. (* returns 3 *)
 
 
 End RaftTestInstance.
