raft/protocols/Raft/RaftContext.v
@@ -1,0 +1,211 @@
+(*! This file is part of the raft implementation with velisarios. !*)
+
+
+(*! Context definitions !*)
+(** This file defines the context, which means the abstract definitions replaced
+ ** by the realization of some program. Also, the definition of a node and the
+ ** realization of a quorum. **)
+Require Export Velisarios.Quorum.
+(* the process module provides the abstraction which is implemented by the protocols *)
+Require Export Velisarios.Process.
+Require Export String.
+
+Section RaftContext.
+
+  (* needed? *)
+  Local Open Scope eo.
+  Local Open Scope proc.
+
+  (*! Context !*)
+  (** The context provides abstract definitions which are replaced by real ones
+   ** within the simulation. **)
+  Class RaftContext :=
+    MkRaftContext
+      {
+        (* number of possible faults *)
+        F : nat;
+        (* number of replicas needed *)
+        num_replicas := (3 * F) + 1;
+
+        (* the replicas are only some type *)
+        Rep : Set;
+        (* replicas have decidable equality *)
+        rep_deq : Deq Rep;
+        (* replicas can be associated with some natural number *)
+        reps2nat : Rep -> nat_n num_replicas;
+        (* the projection is bijective; bijective is defined in Quorum *)
+        reps_bij : bijective reps2nat;
+
+        (* the number of clients allowed *)
+        num_clients : nat;
+        (* clients are just some ordenary type *)
+        Client : Set;
+        (* clients have decidable equality *)
+        client_deq : Deq Client;
+        (* clients can be associated with some number *)
+        clients2nat : Client -> nat_n num_clients;
+        (* the projections ist bijective *)
+        clients_bij : bijective clients2nat;
+
+        (* the content type for the log *)
+        Content : Set;
+        (* get a textual representation from the content *)
+        content2string : Content -> string;
+        (* This is the state of the program to distribute. *)
+        RaftSM : Set;
+        (* the result type which gets issued by the state update function *)
+        RaftSM_result : Set;
+        (* the initial state of the state machine *)
+        RaftSM_initial_state : RaftSM;
+        (* the update function which produces a new state and a result. *)
+        RaftSM_update_state : RaftSM -> Content -> RaftSM * RaftSM_result
+      }.
+  (** To get this construct clear: The proposed functions and types are used by the protocol
+   ** but get instantiated in the RaftSim.v file or some other file which uses the raft protocol. **)
+
+  (** Declares the context type class as new variable with implicit
+   ** generalization of free terms. Since everything is typed no free terms are gneralized? **)
+  Context { raft_context : RaftContext }.
+
+
+  (*! Nodes !*)
+  (** Nodes are used to distinguish between server and clients.
+   ** The parameters are defined in the RaftContext, the real implementation is provided by the simulation. **)
+  Inductive RaftNode :=
+  (* The normal server is a replica which is denoted by the nat/name Rep provided as context information. *)
+  | replica (n : Rep)
+  (* The other node is the client which is in fact not modeled within COQ.
+   * It is modeled in ocaml outside the protocol and only feeds the input. *)
+  | client (n : Client).
+
+  (** Get the replica name/nat of some node. **)
+  Definition replica2rep (n : RaftNode) : option Rep :=
+    match n with
+    | replica n => Some n
+    | _ => None
+    end.
+
+  (** Get the client name/nat of some node. **)
+  Definition client2rep (n : RaftNode) : option Client :=
+    match n with
+    | client n => Some n
+    | _ => None
+    end.
+
+  (** Prove that raft nodes have decidable equality like the one from Leibnitz. **)
+  Lemma RaftnodeDeq : Deq RaftNode.
+  Proof.
+    introv.
+    destruct x as [r1|c1], y as [r2|c2].
+    + destruct (rep_deq r1 r2); [left|right]; subst; auto.
+      intro xx. inversion xx. subst. tcsp.
+    + right; intro xx. inversion xx; subst.
+    + right; intro xx. inversion xx; subst.
+    + destruct (client_deq c1 c2); [left|right]; subst; auto.
+      intro xx. inversion xx. subst. tcsp.
+  Defined.
+
+  (** Bind the real node definition as instance to the abstract definition from velisarios. **)
+  Global Instance Raft_I_Node : Node := MkNode RaftNode RaftnodeDeq.
+
+  (*! Quorum instance !*)
+  (** Replicas are an injective image between names/nats and real implementations **)
+  Lemma replica_inj : injective replica.
+  Proof.
+    introv h. ginv. auto.
+  Qed.
+
+  (** Define a quorum as a set of node names with the property of being
+   ** depictable into the set of natural numbers. **)
+  Global Instance Raft_I_Quorum : Quorum_context :=
+    MkQuorumContext
+      Rep (* the node type *)
+      num_replicas (* size of the set *)
+      rep_deq (* the nodes have to be decidable equality *)
+      reps2nat (* fn which translates nodes to nats *)
+      reps_bij (* node translation is bijective *)
+      replica (* the inductive arm indicates the nodes name *)
+      replica_inj. (* prove that the function is injective *)
+
+  (* can we have something like this?
+   * Since Rep is the node type it would be Rep->Rep *)
+  Definition rep2node := Rep -> node_type.
+
+  (*! More about nodes !*)
+  (* 0 is less than 2*F+1 *)
+  Definition nat_n_2Fp1_0 : nat_n num_replicas.
+  Proof.
+    exists 0.
+    apply leb_correct.
+    unfold num_replicas.
+    omega.
+  Defined.
+
+  Definition replica0 : Rep := bij_inv reps_bij nat_n_2Fp1_0.
+
+  Eval simpl in (name_dec (replica replica0) (replica replica0)).
+
+  (* We'll return the node as given by our bijection if n < num_nodes,
+     otherwise we return a default value (replica0) *)
+  Definition nat2rep (n : nat) : Rep.
+  Proof.
+    destruct reps_bij as [f a b].
+    destruct (lt_dec n num_replicas) as [d|d].
+    - exact (f (mk_nat_n d)). (* here we now that n < num_replicas so we can use our bijection *)
+    - exact replica0. (* here num_replicas <= n, so we return a default value: replica0 *)
+  Defined.
+
+  Definition reps : list Rep := (* list all nodes *)
+   mapin
+      (seq 0 num_replicas)
+      (fun n i => bij_inv reps_bij (mk_nat_n (seq_0_lt i))).
+
+  (* Convert node list to name list *)
+  Definition nreps : list name := map replica reps.
+
+  Lemma reps_prop : forall (x : Rep), In x reps.
+  Proof.
+    exact nodes_prop.
+  Qed.
+
+  Definition clients : list Client := (* list all clients *)
+    mapin
+      (seq 0 num_clients)
+      (fun n i => bij_inv clients_bij (mk_nat_n (seq_0_lt i))).
+
+  (* Convert client list to client name list *)
+  Definition nclients : list name := map client clients.
+
+  Lemma clients_prop : forall (x : Client), In x clients.
+  Proof.
+    introv.
+    unfold clients.
+    apply in_mapin.
+
+
+    remember (clients2nat x) as nx.
+    destruct nx as [nx condnx].
+
+    pose proof (leb_complete _ _ condnx) as c.
+
+    assert (In nx (seq O num_clients)) as i.
+    { apply in_seq; omega. }
+
+    exists nx i; simpl.
+
+    unfold mk_nat_n.
+    unfold bij_inv.
+    destruct clients_bij.
+    pose proof (bij_id1 x) as h.
+    rewrite <- Heqnx in h; subst; simpl.
+
+    f_equal; f_equal.
+    apply UIP_dec; apply bool_dec.
+  Qed.
+
+  (*! Utilities !*)
+  (** From the definition that lists all created replicas. **)
+  Definition other_replicas (r : Rep) : list Rep := remove_elt rep_deq r reps.
+  Definition other_names (r : Rep) : list name := map replica (other_replicas r).
+
+End RaftContext.
